proof/src/SPAPISemantics.ec
@@ -105,120 +105,114 @@ theory SinglePartyAPISemantics.
     theory Language <- Language,
     type sideInfo_t = sideInfo_t.
 
-(* multiple steps... *)
-op stepPiter
-  (step: L -> EnvL -> apiRes_data option -> ((L,EnvL) ECall) option)
-  (k:int)
-  (st:(L,EnvL) APIst)
-  : (L,EnvL) APIst option =
-  IntExtra.IterOp.iter k
-    (fun ost => if ost <> None && callSt (oget ost) = None
-              then let st = oget ost in 
-                   let ecall = step (progSt st) (envSt st) (resSt st) in
-                   omap st_from_step ecall else None) (Some st).
+  (** Multiple steps *)
+  op stepPiter
+    (step: L -> EnvL -> apiRes_data option -> ((L,EnvL) ECall) option)
+    (k:int)
+    (st:(L,EnvL) APIst)
+    : (L,EnvL) APIst option =
+    Int.IterOp.iter k
+      (fun ost => if ost <> None && callSt (oget ost) = None
+                  then let st = oget ost in 
+                     let ecall = step (progSt st) (envSt st) (resSt st) in
+                     omap st_from_step ecall else None) (Some st) axiomatized by stepPiterE.
 
-lemma stepPiter0
- (step : L -> EnvL -> apiRes_data option -> ((L,EnvL) ECall) option) 
- (k : int)
- (st : (L,EnvL) APIst) :
- k <= 0 =>
- stepPiter step k st = Some st.
-proof. by move => ?; rewrite /stepPplus iter0. qed.
+  lemma stepPiter0
+    (step : L -> EnvL -> apiRes_data option -> ((L,EnvL) ECall) option) 
+    (k : int) (st : (L,EnvL) APIst) :
+    k <= 0 => stepPiter step k st = Some st.
+  proof. by move => ?; rewrite /stepPplus; smt(stepPiterE iter0). qed.
 
-lemma nosmt stepPiter1  step (st:(L,EnvL) APIst):
- callSt st = None =>
- stepPiter step 1 st
- = omap st_from_step (step (progSt st) (envSt st) (resSt st)).
-proof.
-rewrite /stepPplus /progSt /envSt /resSt.
-by rewrite iter1 /= => ->.
-qed.
+  lemma nosmt stepPiter1  step (st:(L,EnvL) APIst):
+    callSt st = None =>
+    stepPiter step 1 st = omap st_from_step (step (progSt st) (envSt st) (resSt st)).
+  proof.
+    rewrite /stepPplus /progSt /envSt /resSt => *.
+    by rewrite stepPiterE iter1 /= => /#.
+  qed.
 
-lemma nosmt stepPiterS_none  step k (s:(L,EnvL) APIst):
- stepPiter step k s = None =>
- stepPiter step (k+1) s = None.
-proof.
-move => ?; rewrite /progSt /envSt /resSt.
-case: (0 <= k) => E.
- by rewrite IntExtra.IterOp.iterS //= H => *.
-smt(iter0).
-qed.
+  lemma nosmt stepPiterS_none  step k (s:(L,EnvL) APIst):
+    stepPiter step k s = None =>
+    stepPiter step (k+1) s = None.
+  proof.
+    move => ?; rewrite /progSt /envSt /resSt.
+    case: (0 <= k) => E;
+      first by rewrite stepPiterE Int.IterOp.iterS //=; move : H; rewrite stepPiterE => ->.
+   by  smt(stepPiterE iter0).
+  qed.
 
-lemma nosmt stepPiterS_some  step k (s s':(L,EnvL) APIst) x:
- 0 <= k =>
- stepPiter step k s = Some s' =>
- callSt s' = None =>
- step (progSt s') (envSt s') (resSt s') = Some x =>
- stepPiter step (k+1) s = Some (st_from_step x).
-proof.
-move => ???; rewrite /progSt /envSt /resSt.
-rewrite IntExtra.IterOp.iterS //= => *.
-by rewrite /st_from_step  H0 /= H1 H2.
-qed.
+  lemma nosmt stepPiterS_some  step k (s s':(L,EnvL) APIst) x:
+    0 <= k =>
+    stepPiter step k s = Some s' =>
+    callSt s' = None =>
+    step (progSt s') (envSt s') (resSt s') = Some x =>
+    stepPiter step (k+1) s = Some (st_from_step x).
+  proof.
+    move => ???; rewrite /progSt /envSt /resSt.
+    rewrite stepPiterE IterOp.iterS //= => *.
+    rewrite /st_from_step. 
+    by move : H0; rewrite stepPiterE => -> /= /#.
+  qed.
 
-lemma nosmt stepPiterS  step k (s : (L,EnvL) APIst):
- 0 <= k =>
- stepPiter step (k+1) s = obind (stepPiter step 1) (stepPiter step k s).
-proof.
-elim/natind: k s => //=; first smt(stepPiter0).
-move=> n Hn IH s H.
-rewrite /stepPiter /= (_:2 = 1+1) 1:/# addzA iterS //= IH //=.
-case: (stepPiter step n s) => //= st'.
-case: (stepPiter step 1 st') => //= st''.
-by rewrite iter1.
-qed.
+  lemma nosmt stepPiterS  step k (s : (L,EnvL) APIst):
+    0 <= k =>
+    stepPiter step (k+1) s = obind (stepPiter step 1) (stepPiter step k s).
+  proof.
+    elim/natind: k s => //=; first smt(stepPiter0).
+    move=> n Hn IH s H.
+    rewrite stepPiterE /= (_:2 = 1+1) 1:/# addzA iterS //=. 
+    by move : IH; rewrite stepPiterE => * //=; smt(stepPiterE iter1).
+  qed.
 
-lemma nosmt stepPiter_lt  step (k i:int) (s s': (L,EnvL) APIst):
- 0 <= i < k =>
- stepPiter step k s <> None =>
- stepPiter step i s = Some s' =>
- stepPiter step 1 s' <> None.
-proof.
-elim/natind: k; first smt().
-move=> n Hn IH H.
-rewrite stepPiterS //.
-case: (i=n) => [->|E].
- by move=> ??; move: H0; rewrite H1.
-pose a:= stepPiter step n s.
-case: {2}a (eq_refl a) => [|a'] Ea //=; rewrite Ea //=.
-move=> *; apply IH; smt(). 
-qed.
+  lemma nosmt stepPiter_lt  step (k i:int) (s s': (L,EnvL) APIst):
+    0 <= i < k =>
+    stepPiter step k s <> None =>
+    stepPiter step i s = Some s' =>
+    stepPiter step 1 s' <> None.
+  proof.
+    elim/natind: k; first smt().
+    move=> n Hn IH H.
+    rewrite stepPiterS //.
+    case: (i=n) => [->|E]; first by move=> ??; move: H0; rewrite H1.
+    pose a:= stepPiter step n s.
+    case: {2}a (eq_refl a) => [|a'] Ea //=; rewrite Ea //=.
+    by move=> *; apply IH; smt(). 
+  qed.
 
-lemma callSt_stepPiter  step k (s:(L,EnvL) APIst):
- callSt s <> None =>
- k <= 0 \/ stepPiter step k s = None.
-proof.
-move => ?.
-elim/natind: k.
- by move=> ??; left.
-move=> n Hn [?|?].
- have ->/=: n=0 by smt().
- by rewrite /stepPiter /= iter1 /= H.
-by right; rewrite stepPiterS_none.
-qed.
+  lemma callSt_stepPiter  step k (s:(L,EnvL) APIst):
+    callSt s <> None =>
+    k <= 0 \/ stepPiter step k s = None.
+  proof.
+    move => ?.
+    elim/natind: k; first by move=> ??; left.
+    move=> n Hn [?|?].
+      + have ->/=: n=0 by smt().
+        by rewrite stepPiterE /= iter1 /= H.
+    by right; rewrite stepPiterS_none.
+  qed.
 
-lemma nosmt stepPiter_det  step k1 k2 (s s1' s2': (L,EnvL) APIst):
- 0 <= k1 =>
- 0 <= k2 =>
- stepPiter step k1 s = Some s1' =>
- callSt s1' <> None =>
- stepPiter step k2 s = Some s2' =>
- callSt s2' <> None =>
- k1 = k2.
-proof.
-move => *.
-case: (k1=k2) => // E.
-case: (k1 < k2) => Hlt.
- move: (stepPiter_lt step k2 k1 s s1' _ _ _); first 3 smt().
- move: (callSt_stepPiter step k1 _ H2) => [?|?].
-  move: H1; rewrite (_:k1=0) 1:/# stepPiter0 // => /someI ?.
-  smt(callSt_stepPiter).
- smt(callSt_stepPiter).
-move: (stepPiter_lt step k1 k2 s s2' _ _ _); first 3 smt().
-move: (callSt_stepPiter step k2 _ H4) => [?|?].
- move: H3; rewrite (_:k2=0) 1:/# stepPiter0 // => /someI ?.
- smt(callSt_stepPiter).
-smt(callSt_stepPiter).
-qed.
+  lemma nosmt stepPiter_det  step k1 k2 (s s1' s2': (L,EnvL) APIst):
+    0 <= k1 =>
+    0 <= k2 =>
+    stepPiter step k1 s = Some s1' =>
+    callSt s1' <> None =>
+    stepPiter step k2 s = Some s2' =>
+    callSt s2' <> None =>
+    k1 = k2.
+  proof.
+    move => *.
+    case: (k1=k2) => // E.
+    case: (k1 < k2) => Hlt.
+    move: (stepPiter_lt step k2 k1 s s1' _ _ _); first 3 smt().
+      + move: (callSt_stepPiter step k1 _ H2) => [?|?].
+          + move: H1; rewrite (_:k1=0) 1:/# stepPiter0 // => /someI ?.
+            by smt(callSt_stepPiter).
+        by smt(callSt_stepPiter).
+    move: (stepPiter_lt step k1 k2 s s2' _ _ _); first 3 smt().
+    move: (callSt_stepPiter step k2 _ H4) => [?|?].
+      + move: H3; rewrite (_:k2=0) 1:/# stepPiter0 // => /someI ?.
+        by smt(callSt_stepPiter).
+    by smt(callSt_stepPiter).
+  qed.
  
 end SinglePartyAPISemantics.
